src/Helpers_CvmSemantics.v
@@ -31,6 +31,8 @@ Proof.
   induction t; repeat (monad_unfold; simpl in *); intuition.
   - destruct a; monad_unfold; eauto.
     destruct (aspCb ac a p (encodeEvRaw (get_bits e)) (get_bits e)) eqn:E1; simpl in *; eauto.
+    repeat ff.
+    repeat ff.
 
   - (* at case *)
     repeat ff;
@@ -81,7 +83,10 @@ Proof.
     destruct a; (* asp *)
       try destruct a; (* asp params *)    
       try reflexivity; simpl in *.
+
+      monad_unfold.
       repeat ff.
+      
       
   - (* at case *)
   repeat ff;
@@ -263,6 +268,8 @@ Proof.
   - destruct a; monad_simp; invc H; invc H0; eauto;
     destruct (aspCb ac a p (encodeEvRaw (get_bits e)) (get_bits e)); 
     simpl in *; invc H1; invc H2; eauto.
+    repeat ff.
+    repeat ff.
   - 
   repeat ff;
   unfold doRemote_session' in *;
@@ -357,7 +364,9 @@ Proof.
     try (invc H; eauto);
     destruct (aspCb ac a p (encodeEvRaw (get_bits e)) (get_bits e)); 
     monad_simp; invc H1; invc H2; eauto; simpl in *;
-    try (rewrite H3; eauto).
+    try (rewrite H3; eauto); 
+    repeat ff.
+
   -     repeat ff;
   unfold doRemote_session' in *;
   repeat ff;
