src/Manifest_Compiler.v
@@ -27,6 +27,7 @@ Import ListNotations.
   Definition generate_ASP_dispatcher' (al : AM_Library) (am : Manifest) (par : ASP_PARAMS) (p : Plc) (bs : BS) (rawEv : RawEv) :=
         let (aspid, args, plc, targ) := par in
         let abstract_asps := am.(asps) in
+        (* let external_asps := am.(External_ASPS) in *)
         let local_asps_map := al.(Local_ASPS) in
         let shrunk_map : (MapC ASP_ID (ASPCallback CallBackErrors)) := 
         minify_mapC local_asps_map (fun x => if (in_dec_set x abstract_asps) then true else false) in
@@ -91,6 +92,23 @@ Import ListNotations.
         | None => errC Unavailable
           (* (plc_server_cb plc_server_addr p) *)
         end.
+
+(* This function will lookup for either local Plcs to UUID, or pass them off to the Plc Server *)
+Definition generate_external_ASP_dispatcher `{HID : EqClass ID_Type} (al : AM_Library) (am : Manifest) 
+    : PlcCallback :=
+  (* let plc_server_cb := al.(PlcServer_Cb) in *)
+    let external_asp_map := al.(External_ASPS) in
+    let abstract_external_asps := am.(asps_external) in
+    let shrunk_map := 
+      minify_mapD external_asp_map (fun x => if (in_dec_set x abstract_external_asps) then true else false) in
+
+    fun (i : ASP_ID) =>
+      (* check is the plc "p" is local, with a reference *)
+      match (map_get shrunk_map i) with
+      | Some uuid => resultC uuid
+      | None => errC Unavailable
+        (* (plc_server_cb plc_server_addr p) *)
+      end.
       
   (* This function will lookup the PubKey either locally Plc -> PublicKey or pass off to PubKeyServer *)
   Definition generate_PubKey_dispatcher `{HID : EqClass ID_Type} (al : AM_Library) (am : Manifest) 
@@ -132,9 +150,10 @@ Import ListNotations.
   This function will be used in extraction to either dispatch ASPs to the ASP server, or call a local callback *)
   {|
     absMan   := m ;
-    am_clone_addr := (UUID_AM_Clone al) ;
-    aspCb     := (generate_ASP_dispatcher al m) ;
+    am_clone_addr := (UUID_AM_Clone al);
+    aspCb     := (generate_ASP_dispatcher al m);
     app_aspCb := (generate_appraisal_ASP_dispatcher al m);
+    ext_aspCb := (generate_external_ASP_dispatcher al m);
     plcCb     := (generate_Plc_dispatcher al m);
     pubKeyCb  := (generate_PubKey_dispatcher al m);
     uuidCb    := (generate_UUID_dispatcher al m);
